Flapjack.lean
@@ -16,6 +16,7 @@ import Flapjack.PanMemory
 import Flapjack.RiscV.Model
 import Flapjack.RiscV.PanMemory
 import Flapjack.RiscV.PanSemantics
+import Flapjack.RiscV.Allocator
 import Flapjack.RiscV.Backend
 import Flapjack.RiscV.Calls
 import Flapjack.RiscV.Link
